partial_abort/formalization/equivalence.v
@@ -1,0 +1,23 @@
+Require Export well_formed.
+
+
+
+Inductive poolEq : pool -> pool -> Prop :=
+|ParEq : forall T1 T2 T1' T2', poolEq T1 T1' -> poolEq T2 T2' ->
+                               poolEq (Par T1 T2) (Par T1' T2')
+|ThreadEq : forall Hl L L' t, 
+              getList L = getList L' -> poolEq (Single(Hl,L,t)) (Single(Hl,L',t)). 
+
+
+Theorem fullImpliesPartial : forall n H T n' H' T', 
+                               f_step n H T n' H' T' ->
+                               multistep n H T n' H' T'. 
+Proof.
+  intros. induction H0. 
+  {eapply multi_step. 
+
+
+
+
+
+
