partial_abort/formalization/well_formed.v
@@ -62,14 +62,14 @@ Theorem commitWF : forall n H H' Hl Hl' L L' e e' res,
                      commit H (Hl,L,e) H' (Hl',L',e') res ->
                      heapWF n H -> heapWF n Hl -> heapWF n H' /\ heapWF n Hl'. 
 Proof.
-  intros. dependent induction H0. 
+  intros. dependent induction H0; auto. 
   {split; auto. inv H3. eapply IHcommit in H7; eauto. invertHyp. auto. }
-  {inv H4. split; auto. eapply IHcommit in H8; eauto. invertHyp. auto. }
+  {inv H4. split; auto. }
   {inv H2. split; auto. constructor; auto. eapply IHcommit in H6; eauto.
    invertHyp. auto. }
   {inv H2. split; auto. constructor; auto. eapply IHcommit in H6; eauto. 
    invertHyp. auto. }
-  {inv H2. split; auto. eapply IHcommit in H6; eauto. invertHyp. auto. }
+  {inv H2. eapply IHcommit in H6; eauto. }
 Qed. 
 
 Theorem stepWF : forall n n' H T H' T', 
@@ -106,4 +106,44 @@ Proof.
 Qed. 
 
 
+Theorem commit_fWF : forall n H0 H H' Hl Hl' L L' e e' res, 
+                     commit_f H0 H (Hl,L,e) H' (Hl',L',e') res -> heapWF n H0 ->
+                     heapWF n H -> heapWF n Hl -> heapWF n H' /\ heapWF n Hl'. 
+Proof.
+  intros. dependent induction H1; auto. 
+  {split; auto. inv H5. eapply IHcommit_f in H9; eauto. invertHyp. auto. }
+  {inv H4. split; auto. constructor; auto. eapply IHcommit_f in H8; eauto.
+   invertHyp. auto. }
+  {inv H4. split; auto. constructor; auto. eapply IHcommit_f in H8; eauto.
+   invertHyp. auto. }
+Qed. 
+
+Theorem f_heapCountMonotonic : forall n n' H T H' T', 
+                               f_step n H T n' H' T' -> n' >= n. 
+Proof.
+  intros. induction H0; auto. Qed. 
+
+Theorem f_stepWF : forall n n' H T H' T', 
+                   heapWF n H  -> poolWF n T -> f_step n H T n' H' T' ->
+                   heapWF n' H' /\ poolWF n' T'. 
+Proof. 
+  intros. induction H2; try solve[split; auto; solveLocalHeap]. 
+  {inv H1. apply IHf_step in H5; auto. invertHyp. split; auto. 
+   constructor. auto. eapply poolWFWeakening; eauto. eapply f_heapCountMonotonic; eauto. }
+  {inv H1. apply IHf_step in H6; auto. invertHyp. split; auto. 
+   constructor; auto. eapply poolWFWeakening; eauto. eapply f_heapCountMonotonic; eauto. }
+  {apply IHf_step in H0. invertHyp. split; auto. constructor. inv H5. auto. constructor. 
+   inv H1. auto. }
+  {split. auto. constructor. constructor. inv H1. auto. eapply lookupWF; eauto. }
+  {split. constructor. auto. eapply lookupWF; eauto. solveLocalHeap. }
+  {split. auto. solveLocalHeap. constructor. auto. eapply lookupWF. eapply H0. eauto. }
+  {split; auto. solveLocalHeap. constructor. auto. eapply lookupWF; eauto. }
+  {split. constructor. eapply heapWFWeakening; eauto; omega. omega. solveLocalHeap. 
+   eapply heapWFWeakening; eauto. }
+  {split. eapply heapWFWeakening; eauto. solveLocalHeap. constructor. 
+   eapply heapWFWeakening; eauto. omega. }
+  {eapply commit_fWF in H2; eauto. invertHyp. split. auto. constructor. constructor.
+   inv H1. auto. }
+  {inv H1. eapply commit_fWF in H2; eauto. invertHyp. split; auto. }
+Qed. 
 
